tla-tree/ImmutableDiskTreeHeight.dfy
@@ -1,28 +1,42 @@
 include "ImmutableDiskTreeInv.dfy"
-include "CrashableMap.dfy"
 
-module RefinementProof {
-import opened KVTypes
+module ImmutableDiskTreeHeight {
+import opened TreeTypes
 import opened ImmutableDiskTree
 import opened ImmutableDiskTreeInv
 import opened MissingLibrary
-import CrashableMap
 
-function NodeAt(k:Constants, table:Table, view:View, addr:int) : Node
-    requires PlausibleDiskSize(k)
-    requires WFTable(k, table)
-    requires AllocatedNbasValid(k, table)
-    requires addr in AllocatedAddresses(k, table)
-    requires FullView(k, view)
+// A view of a thing we expect to be a tree -- but at this point we're still proving it.
+// So it's just a "graph" for now.
+datatype GraphView = GraphView(k:Constants, table:Table, view:View)
+
+predicate SaneTableInView(gv:GraphView)
 {
-    var nba := table[addr];
-    var lba := LbaForNba(k, nba);
-    var sector := view[lba];
+    && PlausibleDiskSize(gv.k)
+    && WFTable(gv.k, gv.table)
+    && AllocatedNbasValid(gv.k, gv.table)
+    && FullView(gv.k, gv.view)
+    && TableBlocksTypeCorrect(gv.k, gv.view)
+    && AllocatedNodeBlocksTypeCorrect(gv.k, gv.view, gv.table)
+}
+
+predicate SaneNodeInView(gv:GraphView, addr:TableAddress)
+{
+    && SaneTableInView(gv)
+    && addr in AllocatedAddresses(gv.k, gv.table)
+}
+
+function NodeAt(gv:GraphView, addr:TableAddress) : Node
+    requires SaneNodeInView(gv, addr)
+{
+    var nba := TableAt(gv.k, gv.table, addr);
+    var lba := LbaForNba(gv.k, nba);
+    var sector := gv.view[lba];
     sector.node
 }
 
 type Height = Option<int>
-type AddrHeightMap = map<int,int>   // Maps from addresses to height of the tree at that address. Zero is an Unused addr.
+type AddrHeightMap = map<TableAddress,int>   // Maps from addresses to height of the tree at that address. Zero is an Unused addr.
 
 predicate LeafNode(node:Node)
 {
@@ -44,6 +58,7 @@ predicate HeightAtMost(height:Height, bound:int)
 }
 
 predicate AllSlotHeightsAtMost(node:Node, heightMap:AddrHeightMap, slotCount:int, bound:int)
+    requires slotCount <= |node.slots|
 {
     forall i :: 0<=i<slotCount ==> HeightAtMost(HeightForSlot(node.slots[i], heightMap), bound)
 }
@@ -56,7 +71,12 @@ function CombineHeights(h1:Height, h2:Height) : Height
 }
 
 function {:opaque} DefineHeightNonLeafPrefix(node:Node, heightMap:AddrHeightMap, slotCount:int) : (h:Height)
+    requires 0<=slotCount<=|node.slots|
     ensures h.Some? ==> AllSlotHeightsAtMost(node, heightMap, slotCount, h.value)
+    ensures h.Some? ==> 0<=h.value
+    ensures h.Some? ==> forall slotIdx
+        :: ValidSlotIndex(node, slotIdx) && slotIdx < slotCount && node.slots[slotIdx].Pointer?
+        ==> node.slots[slotIdx].addr in heightMap
 {
     if slotCount==0
     then Some(1)
@@ -66,114 +86,171 @@ function {:opaque} DefineHeightNonLeafPrefix(node:Node, heightMap:AddrHeightMap,
             HeightForSlot(node.slots[slotCount-1], heightMap))
 }
 
-function DefineHeightAddr(k:Constants, table:Table, view:View, heightMap:AddrHeightMap, addr:int) : (h:Height)
+function DefineHeightAddr(gv:GraphView, heightMap:AddrHeightMap, addr:TableAddress) : (h:Height)
+    requires SaneNodeInView(gv, addr)
     ensures h.Some? ==> 0<=h.value
 {
-    if table[addr].Unused?
+    if TableAt(gv.k, gv.table, addr).Unused?
     then Some(0)
     else
-        var node := NodeAt(k, table, view, addr);
+        var node := NodeAt(gv, addr);
         DefineHeightNonLeafPrefix(node, heightMap, |node.slots|)
 
 }
 
-function {:opaque} SlotHeightMapDef(k:Constants, table:Table, view:View, maxHeight:int) : AddrHeightMap
+predicate WFHeightMap(heightMap:AddrHeightMap)
+{
+    forall addr :: addr in heightMap ==> 0 <= heightMap[addr]
+}
+
+predicate HeightMapNests(gv:GraphView, heightMap:AddrHeightMap)
+    requires SaneTableInView(gv)
+{
+    forall addr, idx :: (
+            && addr in AllocatedAddresses(gv.k, gv.table)
+            && addr in heightMap
+            && ValidSlotIndex(NodeAt(gv, addr), idx)
+            && NodeAt(gv, addr).slots[idx].Pointer?
+        ) ==> NodeAt(gv, addr).slots[idx].addr in heightMap
+}
+
+predicate HeightMapDecreases(gv:GraphView, heightMap:AddrHeightMap)
+    requires SaneTableInView(gv)
+    requires HeightMapNests(gv, heightMap)
+{
+    forall addr, idx :: (
+            && addr in AllocatedAddresses(gv.k, gv.table)
+            && addr in heightMap
+            && ValidSlotIndex(NodeAt(gv, addr), idx)
+            && NodeAt(gv, addr).slots[idx].Pointer?
+        ) ==> heightMap[NodeAt(gv, addr).slots[idx].addr] < heightMap[addr]
+}
+
+function {:opaque} SlotHeightMapDef(gv:GraphView, maxHeight:int) : (heightMap:AddrHeightMap)
+    requires 0<=maxHeight
+    requires SaneTableInView(gv)
+    ensures WFHeightMap(heightMap)
 {
     if maxHeight == 0
     then
-        map addr | addr in ValidAddresses(k) && table[addr].Used? :: 0
+        map addr | addr in ValidAddresses(gv.k) && TableAt(gv.k, gv.table, addr).Unused? :: 0
     else
         map addr | 
-            addr in ValidAddresses(k)
-            && DefineHeightAddr(k, table, view, SlotHeightMapDef(k, table, view, maxHeight-1), addr).Some?
-            :: DefineHeightAddr(k, table, view, SlotHeightMapDef(k, table, view, maxHeight-1), addr).value
+            && addr in AllocatedAddresses(gv.k, gv.table)
+            && DefineHeightAddr(gv, SlotHeightMapDef(gv, maxHeight-1), addr).Some?
+            :: DefineHeightAddr(gv, SlotHeightMapDef(gv, maxHeight-1), addr).value
 }
 
-function SlotHeightMap(k:Constants, table:Table, view:View) : AddrHeightMap
+lemma
+    DefineHeightAddr(gv, SlotHeightMapDef(gv, maxHeight-1), addr).Some?
+    ==> DefineHeightAddr(gv, SlotHeightMapDef(gv, maxHeight), addr).Some?
+
+Okay, brain.
+At maxheight 0, there's some stuff in the table (unused addrs).
+At maxheight 1, all those things are in the table (DefineHeightAddr defn), plus things defined by
+DefineHeightNonLeafPrefix.
+At maxheight 2, some new things are in the table, but everything that was in the table before is still
+in there for the same reason it was before.
+
+lemma HeightMapMonotonic(gv:GraphView, maxHeight:int)
+    requires SaneTableInView(gv)
+    requires 0 < maxHeight
+    ensures SlotHeightMapDef(gv, maxHeight-1).Keys <= SlotHeightMapDef(gv, maxHeight).Keys
 {
-    SlotHeightMapDef(k, table, view, k.tableEntries)
+    reveal_SlotHeightMapDef();
+    var lo := SlotHeightMapDef(gv, maxHeight-1);
+    var hi := SlotHeightMapDef(gv, maxHeight);
+    forall addr | addr in lo
+        ensures addr in hi
+    {
+        if (maxHeight == 1) {
+            assert addr in ValidAddresses(gv.k);
+            assert TableAt(gv.k, gv.table, addr).Unused?;
+            assert addr in hi;
+        } else {
+            assert addr in AllocatedAddresses(gv.k, gv.table)
+           assert DefineHeightAddr(gv, SlotHeightMapDef(gv, maxHeight-2), addr).Some?
+            HeightMapMonotonic(gv, lo-1, addr);
+            assert addr in hi;
+        }
+    }
 }
 
-// If there are no cycles, then every address can be assigned a height.
-predicate CycleFree(k:Constants, heightMap:AddrHeightMap)
+lemma SlotHeightMapDefProperties(gv:GraphView, maxHeight:int, heightMap:AddrHeightMap)
+    requires 0<=maxHeight
+    requires SaneTableInView(gv)
+    requires SlotHeightMapDef(gv, maxHeight) == heightMap
+    ensures HeightMapNests(gv, heightMap)
+    ensures HeightMapDecreases(gv, heightMap)
+{
+    reveal_SlotHeightMapDef();
+    forall addr, idx | (
+            && addr in AllocatedAddresses(gv.k, gv.table)
+            && addr in heightMap
+            && ValidSlotIndex(NodeAt(gv, addr), idx)
+            && NodeAt(gv, addr).slots[idx].Pointer?
+        ) 
+        ensures NodeAt(gv, addr).slots[idx].addr in heightMap
+    {
+        assert addr in heightMap;
+        var node := NodeAt(gv, addr);
+        if (maxHeight == 0) {
+            assert node.slots[idx].addr in heightMap;
+        } else {
+            var subhm := SlotHeightMapDef(gv, maxHeight-1);
+            var dha := DefineHeightAddr(gv, subhm, addr);
+            assert dha.Some?;
+
+            assert dha == if TableAt(gv.k, gv.table, addr).Unused?
+                then Some(0)
+                else
+                    var node := NodeAt(gv, addr);
+                    DefineHeightNonLeafPrefix(node, subhm, |node.slots|);
+
+            if TableAt(gv.k, gv.table, addr).Unused? {
+                assert node.slots[idx].addr in heightMap;
+            } else {
+                assert dha == DefineHeightNonLeafPrefix(node, subhm, |node.slots|);
+                reveal_DefineHeightNonLeafPrefix();
+                assert dha == CombineHeights(
+                    DefineHeightNonLeafPrefix(node, subhm, |node.slots|-1),
+                    HeightForSlot(node.slots[|node.slots|-1], subhm));
+                assert node.slots[idx].addr in subhm;
+                var subaddr := node.slots[idx].addr;
+                SlotHeightMapDefProperties(gv, maxHeight-1, subhm);
+
+                assert subaddr in AllocatedAddresses(gv.k, gv.table);
+                assert subaddr in heightMap;
+                assert ValidSlotIndex(NodeAt(gv, subaddr), idx);
+                assert NodeAt(gv, subaddr).slots[idx].Pointer?;
+
+                assert node.slots[idx].addr in heightMap;
+            }
+        }
+    }
+    assert HeightMapDecreases(gv, heightMap);
+}
+
+function SlotHeightMap(gv:GraphView) : AddrHeightMap
+    requires SaneTableInView(gv)
+{
+    SlotHeightMapDefProperties(gv, gv.k.tableEntries, SlotHeightMapDef(gv, gv.k.tableEntries));
+    SlotHeightMapDef(gv, gv.k.tableEntries)
+}
+
+predicate HeightMapComplete(k:Constants, heightMap:AddrHeightMap)
 {
     heightMap.Keys == ValidAddresses(k)
 }
 
-
-//// left off here
-/*
-
-// The datums at or below slot slotNum of the tree at table[addr].
-function {:opaque} ISlotView(k:Constants, table:Table, view:View, addr:int, slotNum:int) : CrashableMap.View
+// If there are no cycles, then every address can be assigned a height.
+predicate CycleFree(gv:GraphView, heightMap:AddrHeightMap)
 {
-    var node := NodeAt(k, table, view, addr);
-    var slot := node[slotNum];
-    match slot {
-        case Empty => CrashableMap.EmptyMap()
-        case Value(datum) => SingletonMap(datum.key, datum.value)
-        case Pointer(idx) => ITreeView(k, table, view, idx, 
-    if slot.Empty
-    then 
-    els
+    && WFHeightMap(heightMap)
+    && SaneTableInView(gv)
+    && HeightMapNests(gv, heightMap)
+    && HeightMapDecreases(gv, heightMap)
+    && HeightMapComplete(gv.k, heightMap)
 }
-
-// The datums in the first slotCount slots of the tree at table[addr].
-function {:opaque} ISubtreePrefixView(k:Constants, table:Table, view:View, addr:int, slotCount:int) : CrashableMap.View
-{
-    if slotCount==0
-    then CrashableMap.EmptyMap()
-    else JoinMap(ISubtreeView(k, table, view, addr, slotCount - 1), ISlotView(k, table, view, addr, slotCount - 1))
-}
-
-function ISubtreeView(k:Constants, table:Table, view:View, addr:int) : CrashableMap.View
-{
-    var slotCount := |NodeAt(k, table, view, addr).slots|;
-    ISubtreePrefixView(k, table, view, addr, slotCount)
-}
-
-function ITreeView(k:Constants, table:Table, view:View) : CrashableMap.View
-{
-    ISubtreePrefixView(k, table, view, ROOT_ADDR())
-}
-
-function IEphemeralView(k:Constants, s:Variables) : CrashableMap.View
-{
-    ITreeView(k, s.ephemeralTable, ViewOfCache(s.cache))
-}
-
-function PersistentTable(k:Constants, s:Variables) : Table
-    requires ValidDiskSize(k, s)
-    requires TableBlocksTypeCorrect(k, s)
-{
-    var super := s.disk.sectors[SUPERBLOCK_LBA()];
-    var ti := super.liveTable;
-    var sectors := s.disk.sectors[TableBegin(k, ti) .. TableBegin(k, ti) + k.tableSectors];
-    UnmarshallTable(k, sectors)
-}
-
-function IPersistentView(k:Constants, s:Variables) : CrashableMap.View
-    requires ValidDiskSize(k, s)
-    requires TableBlocksTypeCorrect(k, s)
-    requires AllocatedNbasValid(k, PersistentTable(k, s))
-    requires PersistentAllocatedNodesTypeCorrect(k, s)
-{
-    ITreeView(k, PersistentTable(k, s), ViewOfDisk(s.disk))
-}
-
-function IViews(k:Constants, s:Variables) : seq<CrashableMap.View>
-    requires Inv(k, s)
-{
-    if s.ready?
-    then [IEphemeralView(k, s), IPersistentView(k, s)]
-    else [IPersistentView(k, s)]
-}
-
-function I(k:Constants, s:Variables) : CrashableMap.Variables
-    requires Inv(k, s)
-{
-    CrashableMap.Variables(IViews(k, s))
-}
-*/
 
 } // module
