tla-tree/MissingLibrary.dfy
@@ -13,6 +13,21 @@ function {:opaque} MapRemove<K,V>(m:map<K,V>, k:K) : (m':map<K,V>)
     map j | j in m && j != k :: m[j]
 }
 
+function {:opaque} SingletonImap<K,V>(k:K, v:V) : (m:imap<K,V>)
+    ensures m.Keys == iset {k}
+    ensures m[k] == v
+{
+    imap j | j == k :: v
+}
+
+function {:opaque} ImapUnionPreferB<U,T>(mapa: imap<U,T>, mapb: imap<U,T>) : (mapc:imap<U,T>)
+    ensures mapc.Keys == mapa.Keys + mapb.Keys;
+    ensures forall k :: k in mapb.Keys ==> mapc[k] == mapb[k];
+    ensures forall k :: k in mapb.Keys - mapa.Keys ==> mapc[k] == mapb[k];
+{
+    imap x : U | (x in mapa.Keys + mapb.Keys) :: if x in mapb then mapb[x] else mapa[x]
+}
+
 datatype Option<V> = None | Some(value:V)
 
 function max(a:int, b:int) : int
